Reorganization

examples/metatheory/stlc_constr_db_par.fst
@@ -16,74 +16,12 @@
 
 module StlcConstrDeBruijnParallelSub
 
-type ty =
-  | TArrow : t1:ty -> t2:ty -> ty
+(* Constructive style progress and preservation proof for STLC with
+   CBV reduction, using deBruijn indices and parallel substitution.
+   An awkward special case pf stlc_strongred.fst; in fact this proof
+   is _more_ complex than the one in stlc_strongred.fst! *)
 
-type var = nat
-
-type exp =
-  | EVar   : var -> exp
-  | EApp   : exp -> exp -> exp
-  | EAbs   : ty -> exp -> exp
-
-val is_value : exp -> Tot bool
-let is_value = is_EAbs
-
-type sub = var -> Tot exp
-
-(* Parallel substitution operation `subst` *)
-
-(* It would be fun to show this terminating;
-   the usual way is to replace the subst_f part by a "renaming"
-   (function from vars to vars), but we have a super flexible termination
-   machanism, can't we prove this directly? Probably not, one would normally
-   use lexicographic ordering composed of:
-   1) an _undecidable_ well-founded order on substitutions that equates
-      all renamings, equates all non-renamings, and makes renamings
-      strictly smaller than non-renamings; given that our order has to
-      be on values, for which we are constructive, we can't write down
-      a function mapping substitutions (infinite objects)
-      to 0 (renaming) or 1 (non-renaming)
-   2) the structure of the expression e *)
-
-(* My proposal would be to put this in Classic not Tot *)
-assume val excluded_middle : p:Type -> Tot (b:bool{b = true <==> p})
-
-type renaming (s:sub) = (forall (x:var). is_EVar (s x))
-
-val is_renaming : s:sub -> Tot (n:int{(renaming s ==> n=0) /\
-                                      (~(renaming s) ==> n=1)})
-let is_renaming s = (if excluded_middle (renaming s) then 0 else 1)
-(* Patterns are incomplete? WTF? Filed as #122 *)
-
-val inc_var : var -> Tot exp
-let inc_var y = EVar (y+1)
-
-val renaming_inc_var : unit -> Lemma (renaming (inc_var))
-let renaming_inc_var _ = ()
-
-val subst : e:exp -> s:sub -> Tot exp (decreases %[is_renaming s; e])
-val subst_eabs : sub -> Tot sub
-let rec subst e s =
-  match e with
-  | EVar x -> s x
-  | EAbs t e1 -> EAbs t (subst e1 (subst_eabs s))
-  | EApp e1 e2 -> EApp (subst e1 s) (subst e2 s)
-and subst_eabs s =
-  fun y -> if y = 0 then EVar y
-           else subst (s (y-1)) inc_var
-
-(* subst_beta_gen is a generalization of the substitution we do for the beta rule,
-   when we've under x binders (useful for the substitution lemma) *)
-val subst_beta_gen_aux : var -> exp -> Tot sub
-let subst_beta_gen_aux x v = fun y -> if y < x then (EVar y)
-                                      else if y = x then v
-                                      else (EVar (y-1))
-
-val subst_beta_gen : var -> exp -> exp -> Tot exp
-let subst_beta_gen x v e = subst e (subst_beta_gen_aux x v)
-
-let subst_beta v e = subst_beta_gen 0 v e
+open StlcStrongRed
 
 val step : exp -> Tot (option exp)
 let rec step e =
@@ -104,35 +42,6 @@ let rec step e =
         | None     -> None)
   | _ -> None
 
-type env = var -> Tot (option ty)
-
-val empty : env
-let empty _ = None
-
-val extend : env -> var -> ty -> Tot env
-let extend g x t y = if y < x then g y 
-                     else if y = x then Some t
-                     else g (y-1)
-
-type rtyping : env -> exp -> ty -> Type =
-  | TyVar : #g:env ->
-            x:var{is_Some (g x)} ->
-              rtyping g (EVar x) (Some.v (g x))
-  | TyAbs : #g:env ->
-            t:ty ->
-            #e1:exp ->
-            #t':ty ->
-            rtyping (extend g 0 t) e1 t' ->
-            rtyping g (EAbs t e1) (TArrow t t')
-  | TyApp : #g:env ->
-            #e1:exp ->
-            #e2:exp ->
-            #t11:ty ->
-            #t12:ty ->
-            rtyping g e1 (TArrow t11 t12) ->
-            rtyping g e2 t11 ->
-            rtyping g (EApp e1 e2) t12
-
 val progress : #e:exp -> #t:ty -> h:rtyping empty e t ->
       Lemma (ensures (is_value e \/ (is_Some (step e)))) (decreases h)
 let rec progress _ _ h =
@@ -141,12 +50,6 @@ let rec progress _ _ h =
   | TyAbs _ _ -> ()
   | TyApp h1 h2 -> progress h1; progress h2
 
-val appears_free_in : x:var -> e:exp -> Tot bool (decreases e)
-let rec appears_free_in x e =
-  match e with
-  | EVar y -> x = y
-  | EApp e1 e2 -> appears_free_in x e1 || appears_free_in x e2
-  | EAbs _ e1 -> appears_free_in (x+1) e1
 
 val free_in_context : x:var -> #e:exp -> #g:env -> #t:ty -> h:rtyping g e t ->
       Lemma (ensures (appears_free_in x e ==> is_Some (g x))) (decreases h)
@@ -204,26 +107,7 @@ val typable_empty_closed : #e:exp -> #t:ty -> h:rtyping empty e t ->
       Lemma (ensures (closed e))
 let typable_empty_closed e t h = typable_below 0 h
 
-opaque logic type Equal (g1:env) (g2:env) =
-                 (forall (x:var). g1 x = g2 x)
-opaque logic type EqualE (e:exp) (g1:env) (g2:env) =
-                 (forall (x:var). appears_free_in x e ==> g1 x = g2 x)
 
-val context_invariance : #e:exp -> #g:env -> #t:ty -> 
-      h:(rtyping g e t) -> g':env{EqualE e g g'} ->
-      Tot (rtyping g' e t) (decreases h)
-let rec context_invariance _ _ _ h g' =
-  match h with
-  | TyVar x -> TyVar x
-  | TyAbs t_y h1 ->
-    TyAbs t_y (context_invariance h1 (extend g' 0 t_y))
-  | TyApp h1 h2 ->
-    TyApp (context_invariance h1 g') (context_invariance h2 g')
-
-val typing_extensional : #e:exp -> #g:env -> #t:ty ->
-      h:(rtyping g e t) -> g':env{Equal g g'} ->
-      Tot (rtyping g' e t)
-let typing_extensional _ _ _ h g' = context_invariance h g'
 
 val subst_gen_var_lt : x:var -> y:var{y < x} -> v:exp -> Lemma
   (ensures (subst_beta_gen x v (EVar y) = (EVar y)))
@@ -274,27 +158,11 @@ let subst_gen_eabs_aux x v y =
              subst_closed v inc_var)
      else ())
 
-opaque logic type SubEqual (s1:sub) (s2:sub) =
-                 (forall (x:var). s1 x = s2 x)
-
 val subst_gen_eabs_aux_forall : x:var -> v:exp{closed v} -> Lemma
       (ensures (SubEqual (subst_eabs (subst_beta_gen_aux  x    v))
                                      (subst_beta_gen_aux (x+1) v)))
 let subst_gen_eabs_aux_forall x v = admit()
 (* should follow from subst_gen_eabs_aux and forall_intro *)
-
-val subst_extensional: s1:sub -> s2:sub{SubEqual s1 s2} -> e:exp -> Lemma
-      (subst e s1 = subst e s2) (decreases e)
-(*      [SMTPat [subst e s1; subst e s2]] -- fails type-checking *)
-(* the proof should be trivial with the extensionality axiom *)
-let rec subst_extensional s1 s2 e =
-  match e with
-  | EVar x -> ()
-  | EAbs t e1 -> subst_extensional (subst_eabs s1)
-                                   (subst_eabs s2) e1;
-                 assert(subst (EAbs t e1) s1 =
-                          EAbs t (subst e1 (subst_eabs s1)))
-  | EApp e1 e2 -> (subst_extensional s1 s2 e1; subst_extensional s1 s2 e2)
 
 val subst_gen_eabs : x:var -> v:exp{closed v} -> t_y:ty -> e':exp -> Lemma
       (ensures (subst_beta_gen x v (EAbs t_y e') =
