examples/metatheory/stlc_fullred.fst
@@ -14,9 +14,82 @@
    limitations under the License.
 *)
 
-module StlcFullRed
+module StlcStrongRed
 
-open StlcConstrDeBruijnParallelSub
+(* Constructive-style progress and preservation proof for STLC with
+   strong reduction, using deBruijn indices and parallel substitution. *)
+
+type ty =
+  | TArrow : t1:ty -> t2:ty -> ty
+
+type var = nat
+
+type exp =
+  | EVar   : var -> exp
+  | EApp   : exp -> exp -> exp
+  | EAbs   : ty -> exp -> exp
+
+val is_value : exp -> Tot bool
+let is_value = is_EAbs
+
+(* Parallel substitution operation `subst` *)
+
+(* It would be fun to show this terminating;
+   the usual way is to replace the subst_f part by a "renaming"
+   (function from vars to vars), but we have a super flexible termination
+   machanism, can't we prove this directly? Probably not, one would normally
+   use lexicographic ordering composed of:
+   1) an _undecidable_ well-founded order on substitutions that equates
+      all renamings, equates all non-renamings, and makes renamings
+      strictly smaller than non-renamings; given that our order has to
+      be on values, for which we are constructive, we can't write down
+      a function mapping substitutions (infinite objects)
+      to 0 (renaming) or 1 (non-renaming)
+   2) the structure of the expression e *)
+
+(* My proposal would be to put this in Classic not Tot *)
+assume val excluded_middle : p:Type -> Tot (b:bool{b = true <==> p})
+
+type sub = var -> Tot exp
+
+type renaming (s:sub) = (forall (x:var). is_EVar (s x))
+
+val is_renaming : s:sub -> Tot (n:int{(renaming s ==> n=0) /\
+                                      (~(renaming s) ==> n=1)})
+let is_renaming s = (if excluded_middle (renaming s) then 0 else 1)
+(* Patterns are incomplete? WTF? Filed as #122 *)
+
+val inc_var : var -> Tot exp
+let inc_var y = EVar (y+1)
+
+val renaming_inc_var : unit -> Lemma (renaming (inc_var))
+let renaming_inc_var _ = ()
+
+val subst : e:exp -> s:sub -> Tot exp (decreases %[is_renaming s; e])
+val subst_eabs : sub -> Tot sub
+let rec subst e s =
+  match e with
+  | EVar x -> s x
+  | EAbs t e1 -> EAbs t (subst e1 (subst_eabs s))
+  | EApp e1 e2 -> EApp (subst e1 s) (subst e2 s)
+and subst_eabs s =
+  fun y -> if y = 0 then EVar y
+           else subst (s (y-1)) inc_var
+
+(* subst_beta_gen is a generalization of the substitution we do for
+   the beta rule, when we've under x binders (useful for the
+   substitution lemma) *)
+val subst_beta_gen_aux : var -> exp -> Tot sub
+let subst_beta_gen_aux x v = fun y -> if y < x then (EVar y)
+                                      else if y = x then v
+                                      else (EVar (y-1))
+
+val subst_beta_gen : var -> exp -> exp -> Tot exp
+let subst_beta_gen x v e = subst e (subst_beta_gen_aux x v)
+
+let subst_beta v e = subst_beta_gen 0 v e
+
+(* Operational semantics; non-deterministic, so necessarily in inductive form *)
 
 type rstep : exp -> exp -> Type =
   | SBeta : t:ty ->
@@ -34,6 +107,37 @@ type rstep : exp -> exp -> Type =
             rstep e2 e2' ->
             rstep (EApp e1 e2) (EApp e1 e2')
 
+(* Type system; in inductive form (but not strictly necessary for STLC) *)
+
+type env = var -> Tot (option ty)
+
+val empty : env
+let empty _ = None
+
+val extend : env -> var -> ty -> Tot env
+let extend g x t y = if y < x then g y 
+                     else if y = x then Some t
+                     else g (y-1)
+
+type rtyping : env -> exp -> ty -> Type =
+  | TyVar : #g:env ->
+            x:var{is_Some (g x)} ->
+              rtyping g (EVar x) (Some.v (g x))
+  | TyAbs : #g:env ->
+            t:ty ->
+            #e1:exp ->
+            #t':ty ->
+            rtyping (extend g 0 t) e1 t' ->
+            rtyping g (EAbs t e1) (TArrow t t')
+  | TyApp : #g:env ->
+            #e1:exp ->
+            #e2:exp ->
+            #t11:ty ->
+            #t12:ty ->
+            rtyping g e1 (TArrow t11 t12) ->
+            rtyping g e2 t11 ->
+            rtyping g (EApp e1 e2) t12
+
 (* Defining my own constructive existential *)
 type ex : #a:Type -> (a -> Type) -> Type =
   | ExIntro : #a:Type -> #p:(a -> Type) -> x:a -> p x -> ex p
@@ -47,6 +151,59 @@ let rec progress _ _ h =
      | EAbs t e1' -> ExIntro (subst_beta e2 e1') (SBeta t e1' e2)
      | _          -> (match progress h1 with
                       | ExIntro e1' h1' -> ExIntro (EApp e1' e2) (SApp1 e2 h1'))
+
+(* Subtyping extensional
+   the proof would be trivial with the extensionality axiom *)
+
+opaque logic type SubEqual (s1:sub) (s2:sub) =
+                 (forall (x:var). s1 x = s2 x)
+
+val subst_extensional: s1:sub -> s2:sub{SubEqual s1 s2} -> e:exp -> Lemma
+      (subst e s1 = subst e s2) (decreases e)
+(*      [SMTPat [subst e s1; subst e s2]] -- fails type-checking *)
+let rec subst_extensional s1 s2 e =
+  match e with
+  | EVar x -> ()
+  | EAbs t e1 -> subst_extensional (subst_eabs s1)
+                                   (subst_eabs s2) e1;
+                 assert(subst (EAbs t e1) s1 =
+                          EAbs t (subst e1 (subst_eabs s1)))
+  | EApp e1 e2 -> (subst_extensional s1 s2 e1; subst_extensional s1 s2 e2)
+
+(* Typing extensional (weaker) and context invariance (stronger);
+   they entail lemmas like weakening, strengthening, swapping, etc.
+   Context invariance is actually used in a single place within substitution,
+   for in a specific form of weakening when typing variables. *)
+
+val appears_free_in : x:var -> e:exp -> Tot bool (decreases e)
+let rec appears_free_in x e =
+  match e with
+  | EVar y -> x = y
+  | EApp e1 e2 -> appears_free_in x e1 || appears_free_in x e2
+  | EAbs _ e1 -> appears_free_in (x+1) e1
+
+opaque logic type EqualE (e:exp) (g1:env) (g2:env) =
+                 (forall (x:var). appears_free_in x e ==> g1 x = g2 x)
+opaque logic type Equal (g1:env) (g2:env) =
+                 (forall (x:var). g1 x = g2 x)
+
+val context_invariance : #e:exp -> #g:env -> #t:ty -> 
+      h:(rtyping g e t) -> g':env{EqualE e g g'} ->
+      Tot (rtyping g' e t) (decreases h)
+let rec context_invariance _ _ _ h g' =
+  match h with
+  | TyVar x -> TyVar x
+  | TyAbs t_y h1 ->
+    TyAbs t_y (context_invariance h1 (extend g' 0 t_y))
+  | TyApp h1 h2 ->
+    TyApp (context_invariance h1 g') (context_invariance h2 g')
+
+val typing_extensional : #e:exp -> #g:env -> #t:ty ->
+      h:(rtyping g e t) -> g':env{Equal g g'} ->
+      Tot (rtyping g' e t)
+let typing_extensional _ _ _ h g' = context_invariance h g'
+
+(* Lemmas about substitution bellow lambdas and shifting *)
 
 val inc_var_above : nat -> var -> Tot exp
 let inc_var_above n y = if y<n then EVar y else EVar (y+1)
@@ -95,6 +252,8 @@ let rec typing_shift_up n g v t t' h =
        TyAbs t_y (typing_extensional h21 (extend (extend g n t') 0 t_y)))
   | TyApp h21 h22 -> TyApp (typing_shift_up n t' h21) (typing_shift_up n t' h22)
 
+(* Substitution lemma *)
+
 val substitution_preserves_typing :
       x:var -> #e:exp -> #v:exp -> #t_x:ty -> #t:ty -> #g:env ->
       h1:rtyping g v t_x ->
@@ -116,6 +275,8 @@ let rec substitution_preserves_typing x e v t_x t g h1 h2 =
     (TyApp #g #(subst_beta_gen x v e1) #(subst_beta_gen x v e2) #t11 #t12
        (substitution_preserves_typing x h1 h21)
        (substitution_preserves_typing x h1 h22))
+
+(* Preservation *)
 
 val preservation : #e:exp -> #e':exp -> hs:rstep e e' ->
                    #g:env -> #t:ty -> ht:(rtyping g e t) ->
